chore(library/init/data/list/basic): `mem` => `Mem`

library/init/data/list/basic.lean
@@ -81,23 +81,23 @@ theorem appendAssoc : ∀ (as bs cs : List α), (as ++ bs) ++ cs = as ++ (bs ++ 
   have h₄ : a::(as ++ (bs ++ cs)) = (a::as ++ (bs ++ cs)), from (consAppend a as (bs++cs)).symm,
   Eq.trans (Eq.trans (Eq.trans h₁ h₂) h₃) h₄
 
-inductive mem : α → List α → Prop
-| eqHead (a : α) (as : List α) : mem a (a::as)
-| inTail {a : α} (b : α) {bs : List α} (h : mem a bs) : mem a (b::bs)
+inductive Mem : α → List α → Prop
+| eqHead (a : α) (as : List α) : Mem a (a::as)
+| inTail {a : α} (b : α) {bs : List α} (h : Mem a bs) : Mem a (b::bs)
 
 instance : HasMem α (List α) :=
-⟨List.mem⟩
+⟨Mem⟩
 
 theorem notMem : ∀ {a b : α} {bs : List α}, a ≠ b → ¬ a ∈ bs → ¬ a ∈ b :: bs
-| _ _ _ h _  (mem.eqHead _ _)  := absurd rfl h
-| _ _ _ _ h₁ (mem.inTail _ h₂) := absurd h₂ h₁
+| _ _ _ h _  (Mem.eqHead _ _)  := absurd rfl h
+| _ _ _ _ h₁ (Mem.inTail _ h₂) := absurd h₂ h₁
 
 instance decidableMem [DecidableEq α] (a : α) : ∀ (l : List α), Decidable (a ∈ l)
 | []      := isFalse (λ h, match h with end)
 | (b::bs) :=
-  if h₁ : a = b then isTrue (h₁.symm ▸ mem.eqHead b bs)
+  if h₁ : a = b then isTrue (h₁.symm ▸ Mem.eqHead b bs)
   else match decidableMem bs with
-       | isTrue  h₂ := isTrue (mem.inTail _ h₂)
+       | isTrue  h₂ := isTrue (Mem.inTail _ h₂)
        | isFalse h₂ := isFalse (notMem h₁ h₂)
 
 instance : HasEmptyc (List α) :=
